add: methods of vehicle

source/Vehicle.dfy
@@ -3,27 +3,68 @@ include "Signal.dfy"
 
 // Vehicle class
 class {:autocontracts} Vehicle {
-	var queue : SignalQueue;
+	var queue : PriorityQueue;
 
 	predicate Valid()
 	{
-		true
+		queue.Valid()
+	}
+
+	function sequences() : seq<seq<Signal>>
+	{
+		queue.sequences
 	}
 
 	constructor()
+		ensures sequences() == emptyLists()
 	{
-		queue := new SignalQueue();
+		queue := new PriorityQueue(Reverse(false));
+	}
+
+	function method queueSize() : nat
+		ensures queueSize() == |flatten(sequences())|
+	{
+		queue.size()
+	}
+
+	predicate method emptyQueue()
+		ensures emptyQueue() <==> (queueSize() == 0)
+	{
+		queue.empty()
 	}
 
 	method addSignal(signal : Signal)
+		ensures sequences()[index(getPriority(signal))]
+		== old(sequences()[index(getPriority(signal))]) + [signal]
+		ensures forall k :: 0 <= k < |sequences()| && k != index(getPriority(signal))
+		==> sequences()[k] == old(sequences()[k])
+		ensures queueSize() == old(queueSize()) + 1
 	{
-		queue.add(signal);
+		queue.push(signal, getPriority(signal));
 	}
-
+	
 	method processFirst()
-		requires !queue.empty()
+		requires !queue.empty()		
 	{
 		// Get the first element from the queue
 		var element := queue.pop();
 	}
+
+	function method getFirst() : Signal
+		requires !emptyQueue()
+		ensures getFirst() == sequences()[index(priority(firstNonEmpty(sequences())))][0]
+	{
+		queue.peek()
+	}
+}
+
+method TestVehicle()
+{
+	var v := new Vehicle();
+	assert v.sequences() == [[], [], []];
+	v.addSignal(Reverse(false));
+	assert v.sequences() == [[], [], [Reverse(false)]];
+	v.addSignal(Voltage(30));
+	v.addSignal(Brake(5));
+	assert v.getFirst() == Voltage(30);
 }
